Clean Compiler Model

io/Compiler.Model.fst
@@ -40,96 +40,90 @@ let convert_insts inst_pi spec_pi c1 cmd_call (cmd:io_cmds) arg =
 noeq
 type src_interface = {
   ct : erased tflag -> Type;
-  pt : erased tflag -> Type;
 
   ct_rcs : tree pck_rc;
-  //pt_rc : tree pck_rc;
 
   spec_pi : monitorable_prop;
   inst_pi : monitorable_prop;
   inst_pi_stronger_spec_pi : squash (forall h lt. enforced_locally inst_pi h lt ==> enforced_locally spec_pi h lt);
 
-  //pt_exportable : exportable pt inst_pi pt_rc AllActions;
   ct_importable : fl:erased tflag -> safe_importable (ct fl) spec_pi ct_rcs fl;
+
+  p_post : list string -> trace -> int -> trace -> Type0;
 }
 
 noeq
 type tgt_interface = {
   ct : erased tflag -> Type u#a;
-  pt : Type u#b;
 
   spec_pi : monitorable_prop;
   inst_pi : monitorable_prop;
   inst_pi_stronger_spec_pi : squash (forall h lt. enforced_locally inst_pi h lt ==> enforced_locally spec_pi h lt);
   
-  //pt_ilang : ilang pt inst_pi;
   ct_ilang : fl:erased tflag -> ilang (ct fl) spec_pi;
 }
   
 (** **** languages **)
-
-assume val traces_of : #a:Type -> a ^-> trace_property #IO.Sig.event
+assume val beh : (list string -> IIO int AllActions (fun _ -> True) (fun _ _ _ -> True)) ^-> trace_property #IO.Sig.event
 
 type ctx_src (i:src_interface)  = #fl:erased tflag -> typ_io_cmds fl i.inst_pi -> typ_eff_rcs fl i.ct_rcs -> i.ct fl
-type prog_src (i:src_interface) = #fl:erased tflag -> i.ct (IOActions + fl) -> i.pt (IOActions + fl)
+type prog_src (i:src_interface) = #fl:erased tflag -> i.ct (IOActions + fl) -> argv:list string -> IIO int (IOActions + fl) (fun _ -> True) (i.p_post argv)
+type whole_src = post:(list string -> trace -> int -> trace -> Type0) & (argv:list string -> IIO int AllActions (fun _ -> True) (post argv))
+
+let link_src (#i:src_interface) (p:prog_src i) (c:ctx_src i) : whole_src = 
+  (| i.p_post, p #AllActions (c #AllActions (inst_io_cmds i.inst_pi) (make_rcs_eff i.ct_rcs)) |)
+
+val beh_src : whole_src ^-> trace_property #IO.Sig.event
+let beh_src = on_domain whole_src (fun (| _, ws |) -> beh ws)
 
 let src_language : language = {
   interface = src_interface;
-
-  ctx = ctx_src;
-  pprog = prog_src;
-  whole = (i:src_interface & i.pt AllActions);
-
-  link = (fun #i p c -> 
-    (| i, p #AllActions (c #AllActions (inst_io_cmds i.inst_pi) (make_rcs_eff i.ct_rcs)) |));
-  event_typ = IO.Sig.event;
-
-  beh = (on_domain _ (fun (| i, w |) -> traces_of w)); 
+  ctx = ctx_src; pprog = prog_src; whole = whole_src;
+  link = link_src;
+  event_typ = IO.Sig.event;  beh = beh_src; 
 }
 
 type ctx_tgt (i:tgt_interface) = #fl:erased tflag -> typ_io_cmds fl i.inst_pi -> i.ct fl
-type prog_tgt (i:tgt_interface) = i.ct AllActions -> i.pt
+type prog_tgt (i:tgt_interface) = i.ct AllActions -> list string -> IIO int AllActions (fun _ -> True) (fun _ _ _ -> True)
+type whole_tgt = list string -> IIO int AllActions (fun _ -> True) (fun _ _ _ -> True)
+
+let link_tgt (#i:tgt_interface) (p:prog_tgt i) (c:ctx_tgt i) : whole_tgt =
+  p (c #AllActions (inst_io_cmds i.inst_pi))
+
+val beh_tgt : whole_tgt ^-> trace_property #IO.Sig.event
+let beh_tgt = beh 
 
 let tgt_language : language = {
   interface = tgt_interface;
-
-  ctx = ctx_tgt;
-  pprog = prog_tgt;
-  whole = (i:tgt_interface & i.pt);
-
-  link = (fun #i p c -> (| i, p (c #AllActions (inst_io_cmds i.inst_pi)) |));
-  event_typ = IO.Sig.event;
-
-  beh = (on_domain  (i:tgt_interface & i.pt) (fun (| i, w |) -> traces_of w)); 
+  ctx = ctx_tgt; pprog = prog_tgt; whole = whole_tgt;
+  link = link_tgt;
+  event_typ = IO.Sig.event; beh = beh_tgt; 
 }
 
 (** ** Compile interfaces **)
 let comp_int_src_tgt (i:src_interface) : tgt_interface = {
- // pt = resexn i.pt_exportable.etype;
   ct = (fun fl -> (i.ct_importable fl).sitype);
-  pt = i.pt AllActions;
+
   spec_pi = i.spec_pi;
   inst_pi = i.inst_pi;
   inst_pi_stronger_spec_pi = i.inst_pi_stronger_spec_pi;
 
-//  pt_ilang = ilang_resexn i.inst_pi i.pt_exportable.etype #i.pt_exportable.c_etype;
   ct_ilang = (fun fl -> (i.ct_importable fl).c_sitype);
 }
-
 
 (** ** Compilation **)
 val backtranslate_ctx : (#i:src_interface) -> (c_t:ctx_tgt (comp_int_src_tgt i)) -> src_language.ctx i
 let backtranslate_ctx #i c_t #fl acts eff_rcs =
   (i.ct_importable fl).safe_import (c_t #fl acts) eff_rcs
-  
-val compiler_pprog : (#i:src_interface) -> (p_s:prog_src i) -> tgt_language.pprog (comp_int_src_tgt i)
-let compiler_pprog #i p_s c_t = 
+
+val compile_whole : whole_src -> whole_tgt
+let compile_whole (| _, ws |) = ws
+
+val compile_pprog : (#i:src_interface) -> (p_s:prog_src i) -> prog_tgt (comp_int_src_tgt i)
+let compile_pprog #i p_s c_t = 
   let eff_rcs = make_rcs_eff i.ct_rcs in
   let c_s : i.ct AllActions = (i.ct_importable AllActions).safe_import c_t eff_rcs in
-  let p : i.pt AllActions = p_s #AllActions c_s in
-  // let eff_rc = make_all_rc_eff i.pt_rc in
-  // (i.pt_exportable.export eff_rc p)
-  p
+  p_s #AllActions c_s
 
 let comp : compiler = {
   source = src_language;
@@ -137,18 +131,29 @@ let comp : compiler = {
 
   comp_int = comp_int_src_tgt;
 
-  compile_pprog = compiler_pprog;
+  compile_pprog = compile_pprog;
 
   rel_traces = (==);
 }
 
 (** ** RrHC **)
-let comp_rrhc_2 (i:src_interface) (ct:ctx_tgt (comp_int_src_tgt i)) (ps:prog_src i) : Lemma (
-  let cs : ctx_src i = backtranslate_ctx #i ct in
+let syntactic_equality (i:src_interface) (ct:ctx_tgt (comp_int_src_tgt i)) (ps:prog_src i) : Lemma (
   let it = comp_int_src_tgt i in
-  let pt : prog_tgt it = (compiler_pprog #i ps) in
-  traces_of (ps #AllActions (cs #AllActions (inst_io_cmds i.inst_pi) (make_rcs_eff i.ct_rcs))) ==
-  traces_of (pt (ct #AllActions (inst_io_cmds it.inst_pi)))) = ()
+  let cs : ctx_src i = backtranslate_ctx #i ct in
+  let pt : prog_tgt it = (compile_pprog #i ps) in
+  let wt : whole_tgt = (pt `link_tgt` ct) in
+  let ws : whole_src = (ps `link_src` cs) in
+  compile_whole ws == wt
+) = ()
+  
+let comp_rrhc_2 (i:src_interface) (ct:ctx_tgt (comp_int_src_tgt i)) (ps:prog_src i) : Lemma (
+  let it = comp_int_src_tgt i in
+  let cs : ctx_src i = backtranslate_ctx #i ct in
+  let pt : prog_tgt it = (compile_pprog #i ps) in
+  let wt : whole_tgt = (pt `link_tgt` ct) in
+  let ws : whole_src = (ps `link_src` cs) in
+  beh_src ws == beh_tgt wt) = 
+  syntactic_equality i ct ps
 
 let comp_rrhc_1 (i:comp.source.interface) (ct:comp.target.ctx (comp.comp_int i)) (ps:comp.source.pprog i) : Lemma (
   let cs : comp.source.ctx i = backtranslate_ctx #i ct in
